theories/type_checker_reflects_typing.v
@@ -8,12 +8,25 @@ Set Implicit Arguments.
 Unset Strict Implicit.
 Unset Printing Implicit Defensive.
 
-Require Import operations typing type_checker.
+Require Import common operations typing type_checker.
 
 
 Section Host.
 
 Variable host_function : eqType.
+
+
+Lemma result_typingP : forall r ts,
+  reflect (result_typing r ts) (result_types_agree ts r).
+Proof.
+  move=> + ts. case.
+  - move=> l /=. apply: iffP.
+    + rewrite all2_swap. by apply: all2_mapP.
+    + move=> ?. subst. by constructor.
+    + move=> T. by inversion_clear T.
+  - apply: Bool.ReflectT. by constructor.
+Qed.
+
 
 Lemma wasm_type_checker_reflects_typing:
   forall C (es : function_closure host_function),
